Undo "Remove unused pos argument in memappend_q" per Nickolai's comment:
It certainly seems like [pos] was not pinned down precisely yet, but
if [memappend_q] is not a function of [pos], it seems hard to prove
[wp_txn__doCommit], which will need to prove that [Q pos] holds for an
arbitrary caller-provided [Q].

For example, [Txn.CommitWait] might want to know that, if calls
[txn.log.Flush] on the [n] that it got from [txn.log.MemAppend], its
changes will be made durable.  But if we say nothing about the [pos]
that [Walog.MemAppend] returns, the proof of [wp_txn__doCommit] will
have a hard time proving [Q pos] starting from a [memappend_q ...]
predicate that is not a function of [pos].

src/program_proof/wal/heapspec.v
@@ -261,7 +261,7 @@ Definition memappend_pre γh (bs : list update.t) (olds : list (Block * list Blo
   [∗ list] _ ↦ u; old ∈ bs; olds,
     mapsto (hG := γh) u.(update.addr) 1 (HB (fst old) (snd old)).
 
-Definition memappend_q γh (bs : list update.t) (olds : list (Block * list Block)) : iProp Σ :=
+Definition memappend_q γh (bs : list update.t) (olds : list (Block * list Block)) (pos : u64): iProp Σ :=
   [∗ list] _ ↦ u; old ∈ bs; olds,
     mapsto (hG := γh) u.(update.addr) 1 (HB (fst old) (snd old ++ [u.(update.b)])).
 
@@ -289,12 +289,12 @@ Proof.
   eauto.
 Qed.
 
-Lemma wal_heap_memappend_pre_to_q gh γh bs olds :
+Lemma wal_heap_memappend_pre_to_q gh γh bs olds newpos :
   ( gen_heap_ctx gh ∗
     memappend_pre γh bs olds )
   ==∗
   ( gen_heap_ctx (memappend_gh gh bs olds) ∗
-    memappend_q γh bs olds ).
+    memappend_q γh bs olds newpos ).
 Proof.
   iIntros "(Hctx & Hpre)".
   iDestruct (big_sepL2_length with "Hpre") as %Hlen.
@@ -616,7 +616,7 @@ Qed.
 
 Theorem wal_heap_memappend N2 γh bs (Q : u64 -> iProp Σ) :
   ( |={⊤ ∖ ↑N, ⊤ ∖ ↑N ∖ ↑N2}=> ∃ olds, memappend_pre γh bs olds ∗
-        ( ∀ pos, memappend_q γh bs olds ={⊤ ∖ ↑N ∖ ↑N2, ⊤ ∖ ↑N}=∗ Q pos ) ) -∗
+        ( ∀ pos, memappend_q γh bs olds pos ={⊤ ∖ ↑N ∖ ↑N2, ⊤ ∖ ↑N}=∗ Q pos ) ) -∗
   ( ∀ σ σ' pos,
       ⌜valid_log_state σ⌝ -∗
       ⌜relation.denote (log_mem_append bs) σ σ' pos⌝ -∗
